Added compiler

src/HOL/MicroJava/J/WellType.thy
@@ -96,15 +96,21 @@ apply (rule val.induct)
 apply     auto
 done
 
+lemma typeof_default_val: "\<exists>T. (typeof dt (default_val ty) = Some T) \<and> G\<turnstile> T \<preceq> ty"
+apply (case_tac ty)
+apply (case_tac prim_ty)
+apply auto
+done
+
 types
   java_mb = "vname list \<times> (vname \<times> ty) list \<times> stmt \<times> expr"
 -- "method body with parameter names, local variables, block, result expression."
 -- "local variables might include This, which is hidden anyway"
 
 consts
-  ty_expr :: "java_mb env => (expr      \<times> ty     ) set"
-  ty_exprs:: "java_mb env => (expr list \<times> ty list) set"
-  wt_stmt :: "java_mb env =>  stmt                 set"
+  ty_expr :: "(java_mb env \<times> expr      \<times> ty     ) set"
+  ty_exprs:: "(java_mb env \<times> expr list \<times> ty list) set"
+  wt_stmt :: "(java_mb env \<times> stmt               ) set"
 
 syntax (xsymbols)
   ty_expr :: "java_mb env => [expr     , ty     ] => bool" ("_ \<turnstile> _ :: _"   [51,51,51]50)
@@ -118,11 +124,11 @@ syntax
 
 
 translations
-  "E\<turnstile>e :: T" == "(e,T) \<in> ty_expr  E"
-  "E\<turnstile>e[::]T" == "(e,T) \<in> ty_exprs E"
-  "E\<turnstile>c \<surd>"    == "c     \<in> wt_stmt  E"
+  "E\<turnstile>e :: T" == "(E,e,T) \<in> ty_expr"
+  "E\<turnstile>e[::]T" == "(E,e,T) \<in> ty_exprs"
+  "E\<turnstile>c \<surd>"    == "(E,c)   \<in> wt_stmt"
   
-inductive "ty_expr E" "ty_exprs E" "wt_stmt E" intros
+inductive "ty_expr" "ty_exprs" "wt_stmt" intros
   
   NewC: "[| is_class (prg E) C |] ==>
          E\<turnstile>NewC C::Class C"  -- "cf. 15.8"
@@ -150,7 +156,7 @@ inductive "ty_expr E" "ty_exprs E" "wt_stmt E" intros
   -- "cf. 15.25, 15.25.1"
   LAss: "[| v ~= This;
             E\<turnstile>LAcc v::T;
-      E\<turnstile>e::T';
+            E\<turnstile>e::T';
             prg E\<turnstile>T'\<preceq>T |] ==>
          E\<turnstile>v::=e::T'"
 
@@ -204,6 +210,7 @@ inductive "ty_expr E" "ty_exprs E" "wt_stmt E" intros
            E\<turnstile>s\<surd> |] ==>
         E\<turnstile>While(e) s\<surd>"
 
+
 constdefs
 
  wf_java_mdecl :: "java_mb prog => cname => java_mb mdecl => bool"
@@ -222,9 +229,22 @@ syntax
 translations
   "wf_java_prog" == "wf_prog wf_java_mdecl"
 
+lemma wf_java_prog_wf_java_mdecl: "\<lbrakk> 
+  wf_java_prog G; (C, D, fds, mths) \<in> set G; jmdcl \<in> set mths \<rbrakk>
+  \<Longrightarrow> wf_java_mdecl G C jmdcl"
+apply (simp add: wf_prog_def) 
+apply (simp add: wf_cdecl_def)
+apply (erule conjE)+
+apply (drule bspec, assumption)
+apply simp
+apply (erule conjE)+
+apply (drule bspec, assumption)
+apply (simp add: wf_mdecl_def split_beta)
+done
 
-lemma wt_is_type: "wf_prog wf_mb G \<Longrightarrow> ((G,L)\<turnstile>e::T \<longrightarrow> is_type G T) \<and>  
-       ((G,L)\<turnstile>es[::]Ts \<longrightarrow> Ball (set Ts) (is_type G)) \<and> ((G,L)\<turnstile>c \<surd> \<longrightarrow> True)"
+lemma wt_is_type: "(E\<turnstile>e::T \<longrightarrow> wf_prog wf_mb (prg E) \<longrightarrow> is_type (prg E) T) \<and>  
+       (E\<turnstile>es[::]Ts \<longrightarrow> wf_prog wf_mb (prg E) \<longrightarrow> Ball (set Ts) (is_type (prg E))) \<and> 
+       (E\<turnstile>c \<surd> \<longrightarrow> True)"
 apply (rule ty_expr_ty_exprs_wt_stmt.induct)
 apply auto
 apply (   erule typeof_empty_is_type)
@@ -237,6 +257,6 @@ apply (auto dest!: max_spec2mheads method_wf_mdecl is_type_rTI
             simp add: wf_mdecl_def)
 done
 
-lemmas ty_expr_is_type = wt_is_type [THEN conjunct1,THEN mp, COMP swap_prems_rl]
+lemmas ty_expr_is_type = wt_is_type [THEN conjunct1,THEN mp, rule_format]
 
 end
