src/HOL/MicroJava/BV/Altern.thy
@@ -1,0 +1,67 @@
+
+theory Altern = BVSpec:
+
+
+constdefs
+  check_type :: "jvm_prog \<Rightarrow> nat \<Rightarrow> nat \<Rightarrow> state \<Rightarrow> bool"
+  "check_type G mxs mxr s \<equiv> s \<in> states G mxs mxr"
+
+  wt_instr_altern :: "[instr,jvm_prog,ty,method_type,nat,nat,p_count,
+                exception_table,p_count] \<Rightarrow> bool"
+  "wt_instr_altern i G rT phi mxs mxr max_pc et pc \<equiv>
+  app i G mxs rT pc et (phi!pc) \<and>
+  check_type G mxs mxr (OK (phi!pc)) \<and>
+  (\<forall>(pc',s') \<in> set (eff i G pc et (phi!pc)). pc' < max_pc \<and> G \<turnstile> s' <=' phi!pc')"
+
+  wt_method_altern :: "[jvm_prog,cname,ty list,ty,nat,nat,instr list,
+                 exception_table,method_type] \<Rightarrow> bool"
+  "wt_method_altern G C pTs rT mxs mxl ins et phi \<equiv>
+  let max_pc = length ins in
+  0 < max_pc \<and> 
+  length phi = length ins \<and>
+  check_bounded ins et \<and> 
+  wt_start G C pTs mxl phi \<and>
+  (\<forall>pc. pc<max_pc \<longrightarrow> wt_instr_altern (ins!pc) G rT phi mxs (1+length pTs+mxl) max_pc et pc)"
+
+
+lemma wt_method_wt_method_altern : 
+  "wt_method G C pTs rT mxs mxl ins et phi \<longrightarrow> wt_method_altern G C pTs rT mxs mxl ins et phi"
+apply (simp add: wt_method_def wt_method_altern_def)
+apply (intro strip)
+apply clarify
+apply (drule spec, drule mp, assumption)
+apply (simp add: check_types_def wt_instr_def wt_instr_altern_def check_type_def)
+apply (auto  intro: imageI)
+done
+
+
+lemma check_type_check_types [rule_format]: 
+  "(\<forall>pc. pc < length phi \<longrightarrow> check_type G mxs mxr (OK (phi ! pc)))
+  \<longrightarrow> check_types G mxs mxr (map OK phi)"
+apply (induct phi)
+apply (simp add: check_types_def)
+apply (simp add: check_types_def)
+apply clarify
+apply (frule_tac x=0 in spec)
+apply (simp add: check_type_def)
+apply auto
+done
+
+lemma wt_method_altern_wt_method [rule_format]: 
+  "wt_method_altern G C pTs rT mxs mxl ins et phi \<longrightarrow> wt_method G C pTs rT mxs mxl ins et phi"
+apply (simp add: wt_method_def wt_method_altern_def)
+apply (intro strip)
+apply clarify
+apply (rule conjI)
+  (* show check_types *)
+apply (rule check_type_check_types)
+apply (simp add: wt_instr_altern_def)
+
+  (* show wt_instr *)
+apply (intro strip)
+apply (drule spec, drule mp, assumption)
+apply (simp add: wt_instr_def wt_instr_altern_def)
+done
+
+
+end
