src/HOL/MicroJava/J/Exceptions.thy
@@ -1,0 +1,65 @@
+(*  Title:      HOL/MicroJava/J/Exceptions.thy
+    ID:         $Id$
+    Author:     Gerwin Klein, Martin Strecker
+    Copyright   2002 Technische Universitaet Muenchen
+*)
+
+theory Exceptions = State:
+
+text {* a new, blank object with default values in all fields: *}
+constdefs
+  blank :: "'c prog \<Rightarrow> cname \<Rightarrow> obj"
+  "blank G C \<equiv> (C,init_vars (fields(G,C)))" 
+
+  start_heap :: "'c prog \<Rightarrow> aheap"
+  "start_heap G \<equiv> empty (XcptRef NullPointer \<mapsto> blank G (Xcpt NullPointer))
+                        (XcptRef ClassCast \<mapsto> blank G (Xcpt ClassCast))
+                        (XcptRef OutOfMemory \<mapsto> blank G (Xcpt OutOfMemory))"
+
+
+consts
+  cname_of :: "aheap \<Rightarrow> val \<Rightarrow> cname"
+
+translations
+  "cname_of hp v" == "fst (the (hp (the_Addr v)))"
+
+
+constdefs
+  preallocated :: "aheap \<Rightarrow> bool"
+  "preallocated hp \<equiv> \<forall>x. \<exists>fs. hp (XcptRef x) = Some (Xcpt x, fs)"
+
+lemma preallocatedD:
+  "preallocated hp \<Longrightarrow> \<exists>fs. hp (XcptRef x) = Some (Xcpt x, fs)"
+  by (unfold preallocated_def) fast
+
+lemma preallocatedE [elim?]:
+  "preallocated hp \<Longrightarrow> (\<And>fs. hp (XcptRef x) = Some (Xcpt x, fs) \<Longrightarrow> P hp) \<Longrightarrow> P hp"
+  by (fast dest: preallocatedD)
+
+lemma cname_of_xcp:
+  "raise_if b x None = Some xcp \<Longrightarrow> preallocated hp 
+  \<Longrightarrow> cname_of (hp::aheap) xcp = Xcpt x"
+proof -
+  assume "raise_if b x None = Some xcp"
+  hence "xcp = Addr (XcptRef x)"
+    by (simp add: raise_if_def split: split_if_asm)
+  moreover
+  assume "preallocated hp" 
+  then obtain fs where "hp (XcptRef x) = Some (Xcpt x, fs)" ..
+  ultimately
+  show ?thesis by simp
+qed
+
+lemma preallocated_start:
+  "preallocated (start_heap G)"
+  apply (unfold preallocated_def)
+  apply (unfold start_heap_def)
+  apply (rule allI)
+  apply (case_tac x)
+  apply (auto simp add: blank_def)
+  done
+
+
+
+end
+
